theories/cancellation/MInlineElim.v
@@ -67,7 +67,7 @@ Proof using.
       rewrite SBRed.bind SBRed.vis !vis_trigger. des_ifs; cycle 1.
       { ired. rewrite MIRed.core SBRed.bind SBRed.vis !vis_trigger. des_ifs. cStepS; ss. }
       ired. rewrite MIRed.call. cStepT. rewrite {2}/sandboxed_prog.
-      destruct ((Mod.fnsems md) !! fid fn) eqn:FIND; cycle 1.
+      destruct ((Mod.fnsems md) !! funid fn) eqn:FIND; cycle 1.
       { iApply isim_call_none; eauto. rewrite lookup_fmap FIND //. }
       destruct o; cycle 1.
       { iApply isim_call_none; eauto. rewrite lookup_fmap FIND //. }
@@ -79,7 +79,7 @@ Proof using.
       iPoseProof (winv_split_empty with "[I]") as "[I I']"; et.
       iApply isim_bind. iSplitL "I".
       - cByCoind CIH; et.
-        hexploit (Mod.well_scoped_fns md (fid fn) (msk0, bd0)).
+        hexploit (Mod.well_scoped_fns md (funid fn) (msk0, bd0)).
         { rewrite lookup_omap FIND //. }
         i; ss; des. depdes e; ss. des_ifs.
         { case_bool_decide; eauto. }
